tutorial/lithium/primitive_laws.v
@@ -3,6 +3,7 @@ From iris.base_logic.lib Require Export gen_heap.
 From iris.proofmode Require Import tactics.
 From iris.program_logic Require Import ectx_lifting.
 From lithium.tutorial Require Export lang notation.
+From lithium.tutorial Require Import tactics.
 
 Class tutorialGS (Σ : gFunctors) := TutorialGS {
     tutorial_invGS : invGS Σ;
@@ -19,3 +20,42 @@ Global Instance tutorial_irisG `{!tutorialGS Σ} : irisGS tutorial_lang Σ := {
 
 Notation "l ↦ dq v" := (mapsto l dq v)
   (at level 20, dq custom dfrac at level 1, format "l  ↦ dq  v") : bi_scope.
+
+
+Section lifting.
+  Context `{!tutorialGS Σ}.
+
+  (** Heap *)
+  Lemma wp_alloc s E Φ :
+    (∀ l, l ↦ #0 -∗ Φ (LitV (LitLoc l))) -∗ WP Alloc @ s; E {{ Φ }}.
+  Proof.
+    iIntros "HΦ". iApply wp_lift_atomic_head_step_no_fork; first done.
+    iIntros (σ1 κ κs n nt) "Hσ !>"; iSplit; first by auto with head_step.
+    iIntros "!>" (v2 σ2 efs Hstep) "_Hcred"; inv_head_step.
+    iMod (gen_heap_alloc with "Hσ") as "[Hσ [Hl _]]"; first done.
+    iModIntro; iSplit=> //. iFrame. by iApply "HΦ".
+  Qed.
+
+  Lemma wp_load s E Φ (l : loc) v :
+    l ↦ v -∗ Φ v -∗ WP Load #l @ s; E {{ Φ }}.
+  Proof.
+    iIntros "Hl HΦ". iApply wp_lift_atomic_head_step_no_fork; first done.
+    iIntros (σ1 κ κs n nt) "Hσ !>".
+    iDestruct (gen_heap_valid with "Hσ Hl") as %?.
+    iSplit; first by eauto with head_step.
+    iIntros "!>" (v2 σ2 efs Hstep) "_Hcred"; inv_head_step.
+    iModIntro; iSplit=> //. iFrame.
+  Qed.
+
+  Lemma wp_store s E Φ (l : loc) v (w : val) :
+    l ↦ v -∗ Φ w -∗ WP Store #l w @ s; E {{ Φ }}.
+  Proof.
+    iIntros "Hl HΦ". iApply wp_lift_atomic_head_step_no_fork; first done.
+    iIntros (σ1 κ κs n nt) "Hσ !>".
+    iDestruct (gen_heap_valid with "Hσ Hl") as %?.
+    iSplit; first by eauto with head_step.
+    iIntros "!>" (v2 σ2 efs Hstep) "_Hcred"; inv_head_step.
+    iMod (gen_heap_update with "Hσ Hl") as "[Hσ Hl]".
+    iModIntro; iSplit=> //. iFrame.
+  Qed.
+End lifting.
